ulib/LowStar.Monotonic.Buffer.fsti
@@ -15,7 +15,6 @@
 *)
 module LowStar.Monotonic.Buffer
 
-module P = FStar.Preorder
 module G = FStar.Ghost
 module U32 = FStar.UInt32
 module Seq = FStar.Seq
